Weidenbach_Book/Watched_Literals/Watched_Literals_List_Restart.thy
@@ -2575,7 +2575,7 @@ lemma rtranclp_remove_one_annot_true_clause_count_dec:
   by (induction rule: rtranclp_induct)
     (auto simp: remove_one_annot_true_clause_count_dec)
 
-lemma rtranclp_valid_trail_reduction_count_dec_ge:
+lemma valid_trail_reduction_count_dec_ge:
   \<open>valid_trail_reduction M M' \<Longrightarrow>
     count_decided M' \<le> count_decided M\<close>
   apply (induction rule: valid_trail_reduction.induct)
@@ -2587,7 +2587,7 @@ lemma rtranclp_cdcl_twl_restart_l_count_dec:
     count_decided (get_trail_l S) \<ge> count_decided (get_trail_l b)\<close>
   by (induction rule: cdcl_twl_restart_l.induct)
     (auto simp: remove_one_annot_true_clause_count_dec
-    dest: rtranclp_valid_trail_reduction_count_dec_ge)
+    dest: valid_trail_reduction_count_dec_ge)
 
 lemma remove_one_annot_true_clause_imp_spec:
   assumes
@@ -3400,17 +3400,6 @@ proof -
     done
 qed
 
-
-definition cdcl_twl_full_restart_l_prog where
-\<open>cdcl_twl_full_restart_l_prog S = do {
-   \<comment> \<open> \<^term>\<open>remove_one_annot_true_clause_imp S\<close>\<close>
-    ASSERT(mark_to_delete_clauses_l_pre S);
-    T \<leftarrow> mark_to_delete_clauses_l S;
-    ASSERT (mark_to_delete_clauses_l_post S T);
-    RETURN T
-  }\<close>
-
-
 definition cdcl_GC_clauses_pre :: \<open>'v twl_st_l \<Rightarrow> bool\<close> where
 \<open>cdcl_GC_clauses_pre S \<longleftrightarrow> (
   \<exists>T. (S, T) \<in> twl_st_l None \<and>
@@ -3768,92 +3757,6 @@ definition cdcl_twl_full_restart_l_GC_prog where
     ASSERT(cdcl_twl_restart_l S V);
     RETURN V
   }\<close>
-
-lemma cdcl_twl_full_restart_l_prog_spec:
-  assumes
-    ST: \<open>(S, T) \<in> twl_st_l None\<close> and
-    list_invs: \<open>twl_list_invs S\<close> and
-    struct_invs: \<open>twl_struct_invs T\<close> and
-    confl: \<open>get_conflict_l S = None\<close> and
-    upd: \<open>clauses_to_update_l S = {#}\<close>
-  shows \<open>cdcl_twl_full_restart_l_prog S \<le> \<Down> Id (SPEC(remove_one_annot_true_clause\<^sup>+\<^sup>+ S))\<close>
-proof -
-  have mark_to_delete_clauses_l:
-    \<open>mark_to_delete_clauses_l x \<le> SPEC (\<lambda>T. ASSERT (mark_to_delete_clauses_l_post U T) \<bind>
-             (\<lambda>_. RETURN T)
-             \<le> SPEC (remove_one_annot_true_clause\<^sup>+\<^sup>+ U))\<close>
-    if
-      Ux: \<open>(x, U) \<in> Id\<close> and
-      U: \<open>U \<in> Collect (remove_one_annot_true_clause\<^sup>*\<^sup>* S)\<close>
-      for x U
-  proof -
-    from U have SU: \<open>remove_one_annot_true_clause\<^sup>*\<^sup>* S U\<close> by simp
-    have x: \<open>x = U\<close>
-      using Ux by auto
-    obtain V where
-      SU': \<open>cdcl_twl_restart_l\<^sup>*\<^sup>* S U\<close> and
-      UV: \<open>(U, V) \<in> twl_st_l None\<close> and
-      TV: \<open>cdcl_twl_restart\<^sup>*\<^sup>* T V\<close> and
-      struct_invs_V: \<open>twl_struct_invs V\<close>
-      using rtranclp_remove_one_annot_true_clause_cdcl_twl_restart_l2[OF SU list_invs
-        confl upd ST struct_invs]
-      by auto
-    have
-      confl_U: \<open>get_conflict_l U = None\<close> and
-      upd_U: \<open>clauses_to_update_l U = {#}\<close>
-      using rtranclp_remove_one_annot_true_clause_get_conflict_l[OF SU]
-         rtranclp_remove_one_annot_true_clause_clauses_to_update_l[OF SU] confl upd
-      by auto
-    have list_U: \<open>twl_list_invs U\<close>
-      using SU' list_invs rtranclp_cdcl_twl_restart_l_list_invs by blast
-     have [simp]:
-      \<open>remove_one_annot_true_clause\<^sup>+\<^sup>+ U V' \<Longrightarrow>  mark_to_delete_clauses_l_post U V'\<close> for V'
-      unfolding mark_to_delete_clauses_l_post_def
-      using UV struct_invs_V list_U confl_U upd_U
-      by (blast dest: tranclp_into_rtranclp)
-    show ?thesis
-      unfolding x
-      by (rule mark_to_delete_clauses_l_spec[OF UV list_U struct_invs_V confl_U upd_U,
-         THEN order_trans])
-       (auto intro: RES_refine)
-  qed
-  have 1: \<open>SPEC (remove_one_annot_true_clause\<^sup>*\<^sup>* S) = do {
-       T \<leftarrow> SPEC (remove_one_annot_true_clause\<^sup>*\<^sup>* S);
-       SPEC (remove_one_annot_true_clause\<^sup>*\<^sup>* T)
-    }\<close>
-  by (auto simp: RES_RES_RETURN_RES)
-  have H: \<open>mark_to_delete_clauses_l_pre T\<close>
-    if
-      \<open>(T, U) \<in> Id\<close> and
-      \<open>U \<in> Collect (remove_one_annot_true_clause\<^sup>*\<^sup>* S)\<close>
-    for T U
-  proof -
-    show ?thesis
-      using rtranclp_remove_one_annot_true_clause_cdcl_twl_restart_l2[of S U,
-          OF _ list_invs confl upd ST struct_invs] that list_invs
-      unfolding mark_to_delete_clauses_l_pre_def
-      by (force intro: rtranclp_cdcl_twl_restart_l_list_invs)
-  qed
-  show ?thesis
-    unfolding cdcl_twl_full_restart_l_prog_def
-    apply (refine_vcg mark_to_delete_clauses_l)
-    subgoal
-      using assms
-      unfolding mark_to_delete_clauses_l_pre_def
-      by blast
-    subgoal by auto
-    subgoal by (auto simp: assert_bind_spec_conv)
-    done
-qed
-
-lemma valid_trail_reduction_count_dec_ge:
-  \<open>valid_trail_reduction M M' \<Longrightarrow> count_decided M \<ge> count_decided M'\<close>
-  apply (induction rule: valid_trail_reduction.induct)
-  subgoal for K M M'
-    using trail_renumber_count_dec
-    by (fastforce simp: dest!: get_all_ann_decomposition_exists_prepend)
-  subgoal by (auto dest: trail_renumber_count_dec)
-  done
 
 lemma cdcl_twl_restart_l_count_dec_ge:
   \<open>cdcl_twl_restart_l S T \<Longrightarrow> count_decided (get_trail_l S) \<ge> count_decided (get_trail_l T)\<close>
